AVM/Ecosystem/Translation.lean
@@ -37,3 +37,134 @@ private def logic
   (eco : Ecosystem lab)
   (args : Logic.Args)
   : Bool := sorry
+
+end AVM.Ecosystem
+
+namespace AVM
+
+mutual
+
+partial def Program.tasks
+  {α}
+  {lab : Ecosystem.Label}
+  (eco : Ecosystem lab)
+  (prog : Program lab α)
+  (vals : prog.params.Product)
+  : List Task :=
+  match prog with
+  | .constructor classId constrId args next =>
+    let constr := eco.classes classId |>.constructors constrId
+    let task := constr.task eco args
+    let ⟨newId, vals'⟩ := vals
+    task :: Program.tasks eco (next newId) vals'
+  | .destructor classId destrId selfId args next =>
+    let destr := eco.classes classId |>.destructors destrId
+    let task := destr.task eco selfId args
+    task :: Program.tasks eco next vals
+  | .method classId methodId selfId args next =>
+    let method := eco.classes classId |>.methods methodId
+    let task := method.task eco selfId args
+    task :: Program.tasks eco next vals
+  | .multiMethod methodId selvesIds args next =>
+    let method : MultiMethod methodId := eco.multiMethods methodId
+    let task := method.task eco selvesIds args
+    task :: Program.tasks eco next vals
+  | .fetch _ next =>
+    let ⟨obj, vals'⟩ := vals
+    Program.tasks eco (next obj) vals'
+  | .return _ => []
+
+/-- Creates a Task for a given object constructor. -/
+partial def Class.Constructor.task
+  {lab : Ecosystem.Label}
+  (eco : Ecosystem lab)
+  {classId : lab.ClassId}
+  {constrId : classId.label.ConstructorId}
+  (constr : Class.Constructor classId constrId)
+  (args : constrId.Args.type)
+  : Task :=
+  let bodyParams := (constr.body args).params
+  let params := Program.Parameters.genId (fun _ => bodyParams)
+  Task.absorbParams params fun ⟨newId, vals⟩ =>
+    let body := constr.body args
+    let tasks := Program.tasks eco body vals
+    let newObjData : ObjectData classId.label := body.returnValue vals
+    let newObj : SomeObject :=
+      let obj : Object classId.label :=
+        { uid := newId,
+          nonce := ⟨newId⟩,
+          data := newObjData }
+      obj.toSomeObject
+    let consumedObj := newObj.toConsumable (ephemeral := true)
+    let createdObjects : List CreatedObject :=
+      [CreatedObject.fromSomeObject newObj (ephemeral := false)]
+    Task.composeWithMessage (constr.message ⟨bodyParams.Product⟩ vals newId args) tasks [consumedObj] createdObjects
+
+/-- Creates a Task for a given object destructor. -/
+partial def Class.Destructor.task
+  {lab : Ecosystem.Label}
+  (eco : Ecosystem lab)
+  {classId : lab.ClassId}
+  {destructorId : classId.label.DestructorId}
+  (destructor : Class.Destructor classId destructorId)
+  (selfId : ObjectId)
+  (args : destructorId.Args.type)
+  : Task :=
+  let consumedObjectId : TypedObjectId := ⟨classId.label, selfId⟩
+  let bodyParams (self : Object classId.label) := (destructor.body self args).params
+  let params := Program.Parameters.fetch consumedObjectId bodyParams
+  Task.absorbParams params fun ⟨self, vals⟩ =>
+    let tasks : List Task := Program.tasks eco (destructor.body self args) vals
+    let consumedObj := self.toSomeObject.toConsumable (ephemeral := false)
+    let createdObjects : List CreatedObject :=
+      [{ uid := self.uid,
+         data := self.data,
+         ephemeral := true }]
+    Task.composeWithMessage (destructor.message ⟨(bodyParams self).Product⟩ vals selfId args) tasks [consumedObj] createdObjects
+
+partial def Class.Method.task
+  {lab : Ecosystem.Label}
+  (eco : Ecosystem lab)
+  {classId : lab.ClassId}
+  {methodId : classId.label.MethodId}
+  (method : Class.Method classId methodId)
+  (selfId : ObjectId)
+  (args : methodId.Args.type)
+  : Task :=
+  let consumedObjectId : TypedObjectId := ⟨classId.label, selfId⟩
+  let bodyParams (self : Object classId.label) := (method.body self args).params
+  let params := Program.Parameters.fetch consumedObjectId bodyParams
+  Task.absorbParams params fun ⟨self, vals⟩ =>
+    let body := method.body self args
+    let tasks : List Task := Program.tasks eco body vals
+    let consumedObj := self.toSomeObject.toConsumable (ephemeral := false)
+    let obj := (body.returnValue vals).toSomeObject
+    let createdObjects : List CreatedObject :=
+      [{ uid := obj.object.uid,
+         data := obj.object.data,
+         ephemeral := false }]
+    Task.composeWithMessage (method.message ⟨(bodyParams self).Product⟩ vals selfId args) tasks [consumedObj] createdObjects
+
+partial def MultiMethod.task
+  {lab : Ecosystem.Label}
+  (eco : Ecosystem lab)
+  {methodId : lab.MultiMethodId}
+  (method : MultiMethod methodId)
+  (selvesIds : methodId.SelvesIds)
+  (args : methodId.Args.type)
+  : Task :=
+  let bodyParams (selves : methodId.Selves) : Program.Parameters.{1} := method.body selves args |>.params
+  let params : Program.Parameters.{0} := Program.Parameters.fetchSelves selvesIds bodyParams
+  sorry
+  -- Task.absorbParams params fun (selvesVals : params.Product) =>
+  --   let body := method.body self args
+  --   let tasks : List Task := Program.tasks eco body vals
+  --   let consumedObj := self.toSomeObject.toConsumable (ephemeral := false)
+  --   let obj := (body.returnValue vals).toSomeObject
+  --   let createdObjects : List CreatedObject :=
+  --     [{ uid := obj.object.uid,
+  --        data := obj.object.data,
+  --        ephemeral := false }]
+  --   Task.composeWithMessage (method.message ⟨(bodyParams self).Product⟩ vals selfId args) tasks [consumedObj] createdObjects
+
+end -- mutual
