AVM/Program/Parameters.lean
@@ -1,14 +1,53 @@
 import AVM.Object
+import AVM.Ecosystem.Label
 
 namespace AVM
 
-inductive Program.Parameters where
+inductive Program.Parameters : Type (u + 1) where
   | empty
-  | fetch (param : TypedObjectId) (rest : Object param.classLabel → Program.Parameters)
+  | fetch (param : TypedObjectId.{u}) (rest : Object param.classLabel → Program.Parameters)
   | genId (rest : ObjectId → Program.Parameters)
-deriving Inhabited, Nonempty
+  deriving Inhabited, Nonempty
 
-def Program.Parameters.Product (params : Program.Parameters) : Type u :=
+namespace Program.Parameters
+
+def fetchMany
+  (params : List TypedObjectId)
+  (rest : Pi (params.map (fun param => Object param.classLabel)) Program.Parameters)
+  : Program.Parameters :=
+  match params with
+  | [] => rest.down
+  | i :: is => .fetch i (fun o => fetchMany is (rest o))
+
+-- TODO should this be kept?
+def fetchManyHList
+  (params : List TypedObjectId)
+  (rest : HList (params.map (fun param => Object param.classLabel)) → Program.Parameters)
+  : Program.Parameters := fetchMany params (HList.toPi rest)
+
+theorem helper
+  {lab : Ecosystem.Label}
+  {multiId : lab.MultiMethodId}
+  (selvesIds : multiId.SelvesIds)
+  : HList
+    (List.map (fun param => Object param.classLabel)
+    (List.map (fun arg => { classLabel := arg.classId.label, uid := selvesIds arg : TypedObjectId }) multiId.objectArgNames))
+    =
+    HList (List.map (fun c => Object c.label) multiId.argsClasses) := sorry
+
+def fetchSelves
+  {lab : Ecosystem.Label}
+  {multiId : lab.MultiMethodId}
+  (selvesIds : multiId.SelvesIds)
+  (rest : multiId.Selves → Program.Parameters)
+  : Program.Parameters :=
+    fetchManyHList
+      (multiId.objectArgNames.map (fun arg =>
+                                     { uid := selvesIds arg
+                                       classLabel := arg.classId.label}))
+      (fun h => rest (multiId.SelvesFromHList (helper selvesIds ▸ h)))
+
+def Product (params : Program.Parameters) : Type u :=
   match params with
   | .empty => PUnit
   | .fetch param rest =>
@@ -18,8 +57,6 @@ def Program.Parameters.Product (params : Program.Parameters) : Type u :=
 
 instance {params : Program.Parameters} : TypeRep params.Product where
   rep := Rep.atomic "Program.Parameters.Product" -- TODO: this should depend on params
-
-namespace Program.Parameters
 
 def Product.beq {params : Program.Parameters} (a b : params.Product) :=
     match params with
