Prelude/Function.lean
@@ -1,0 +1,4 @@
+def Pi (ts : List (Type u)) (ret : Type v) : Type (max u v) :=
+  match ts with
+  | .nil => ULift.{u} ret
+  | .cons x xs => x → Pi xs ret
